WIP

code/ecdsa/dist/Hacl_P256.c
@@ -2344,7 +2344,148 @@ static inline void toUint64ChangeEndian_p384(uint8_t *i, uint64_t *o)
   }
 }
 
-static void
+static inline void montgomery_multiplication_buffer_by_one_mixed_p256(uint64_t *result)
+{
+  uint32_t len = (uint32_t)4U;
+  KRML_CHECK_SIZE(sizeof (uint64_t), (uint32_t)2U * len);
+  uint64_t t[(uint32_t)2U * len];
+  memset(t, 0U, (uint32_t)2U * len * sizeof (uint64_t));
+  uint64_t *t_low = t;
+  t_low[0U] = (uint64_t)1U;
+  uint32_t len1 = (uint32_t)4U;
+  for (uint32_t i = (uint32_t)1U; i < len1; i++)
+  {
+    t_low[i] = (uint64_t)0U;
+  }
+  uint32_t len10 = (uint32_t)4U;
+  KRML_CHECK_SIZE(sizeof (uint64_t), (uint32_t)2U * len10);
+  uint64_t t2[(uint32_t)2U * len10];
+  memset(t2, 0U, (uint32_t)2U * len10 * sizeof (uint64_t));
+  for (uint32_t i0 = (uint32_t)0U; i0 < len10; i0++)
+  {
+    uint64_t t10 = t[0U];
+    uint64_t *uu____0 = t2;
+    uint32_t len30 = (uint32_t)4U;
+    for (uint32_t i = (uint32_t)0U; i < len30; i++)
+    {
+      uu____0[i] = (uint64_t)0U;
+    }
+    uint64_t *uu____1 = t2 + (uint32_t)4U;
+    uint32_t len31 = (uint32_t)4U;
+    for (uint32_t i = (uint32_t)0U; i < len31; i++)
+    {
+      uu____1[i] = (uint64_t)0U;
+    }
+    uint64_t temp = (uint64_t)0U;
+    uint64_t f0 = (uint64_t)0xffffffffffffffffU;
+    uint64_t f1 = (uint64_t)0xffffffffU;
+    uint64_t f3 = (uint64_t)0xffffffff00000001U;
+    uint64_t *o0 = t2;
+    uint64_t *o1 = t2 + (uint32_t)1U;
+    uint64_t *o2 = t2 + (uint32_t)2U;
+    uint64_t *o3 = t2 + (uint32_t)3U;
+    uint64_t *o4 = t2 + (uint32_t)4U;
+    mul64(f0, t10, o0, &temp);
+    uint64_t h0 = temp;
+    mul64(f1, t10, o1, &temp);
+    uint64_t l = o1[0U];
+    uint64_t c1 = Lib_IntTypes_Intrinsics_add_carry_u64((uint64_t)0U, l, h0, o1);
+    uint64_t h = temp;
+    o2[0U] = h + c1;
+    mul64(f3, t10, o3, o4);
+    uint32_t len32 = (uint32_t)4U * (uint32_t)2U;
+    uint64_t c = (uint64_t)0U;
+    for (uint32_t i = (uint32_t)0U; i < len32 / (uint32_t)4U * (uint32_t)4U / (uint32_t)4U; i++)
+    {
+      uint64_t t1 = t[(uint32_t)4U * i];
+      uint64_t t210 = t2[(uint32_t)4U * i];
+      uint64_t *res_i0 = t2 + (uint32_t)4U * i;
+      c = Lib_IntTypes_Intrinsics_add_carry_u64(c, t1, t210, res_i0);
+      uint64_t t11 = t[(uint32_t)4U * i + (uint32_t)1U];
+      uint64_t t211 = t2[(uint32_t)4U * i + (uint32_t)1U];
+      uint64_t *res_i1 = t2 + (uint32_t)4U * i + (uint32_t)1U;
+      c = Lib_IntTypes_Intrinsics_add_carry_u64(c, t11, t211, res_i1);
+      uint64_t t12 = t[(uint32_t)4U * i + (uint32_t)2U];
+      uint64_t t212 = t2[(uint32_t)4U * i + (uint32_t)2U];
+      uint64_t *res_i2 = t2 + (uint32_t)4U * i + (uint32_t)2U;
+      c = Lib_IntTypes_Intrinsics_add_carry_u64(c, t12, t212, res_i2);
+      uint64_t t13 = t[(uint32_t)4U * i + (uint32_t)3U];
+      uint64_t t21 = t2[(uint32_t)4U * i + (uint32_t)3U];
+      uint64_t *res_i = t2 + (uint32_t)4U * i + (uint32_t)3U;
+      c = Lib_IntTypes_Intrinsics_add_carry_u64(c, t13, t21, res_i);
+    }
+    for (uint32_t i = len32 / (uint32_t)4U * (uint32_t)4U; i < len32; i++)
+    {
+      uint64_t t1 = t[i];
+      uint64_t t21 = t2[i];
+      uint64_t *res_i = t2 + i;
+      c = Lib_IntTypes_Intrinsics_add_carry_u64(c, t1, t21, res_i);
+    }
+    uint64_t carry = c;
+    uint32_t len3 = (uint32_t)7U;
+    for (uint32_t i = (uint32_t)0U; i < len3; i++)
+    {
+      uint64_t elem = t2[(uint32_t)1U + i];
+      t[i] = elem;
+    }
+    t[len3] = carry;
+  }
+  uint32_t len2 = (uint32_t)4U;
+  uint64_t cin = t[len2];
+  uint64_t *x_ = t;
+  uint32_t len3 = (uint32_t)4U;
+  KRML_CHECK_SIZE(sizeof (uint64_t), len3);
+  uint64_t tempBuffer[len3];
+  memset(tempBuffer, 0U, len3 * sizeof (uint64_t));
+  uint64_t tempBufferForSubborrow = (uint64_t)0U;
+  uint64_t
+  p[4U] =
+    {
+      (uint64_t)0xffffffffffffffffU,
+      (uint64_t)0xffffffffU,
+      (uint64_t)0U,
+      (uint64_t)0xffffffff00000001U
+    };
+  uint32_t len4 = (uint32_t)4U;
+  uint64_t c = (uint64_t)0U;
+  for (uint32_t i = (uint32_t)0U; i < len4 / (uint32_t)4U * (uint32_t)4U / (uint32_t)4U; i++)
+  {
+    uint64_t t1 = x_[(uint32_t)4U * i];
+    uint64_t t210 = p[(uint32_t)4U * i];
+    uint64_t *res_i0 = tempBuffer + (uint32_t)4U * i;
+    c = Lib_IntTypes_Intrinsics_sub_borrow_u64(c, t1, t210, res_i0);
+    uint64_t t10 = x_[(uint32_t)4U * i + (uint32_t)1U];
+    uint64_t t211 = p[(uint32_t)4U * i + (uint32_t)1U];
+    uint64_t *res_i1 = tempBuffer + (uint32_t)4U * i + (uint32_t)1U;
+    c = Lib_IntTypes_Intrinsics_sub_borrow_u64(c, t10, t211, res_i1);
+    uint64_t t11 = x_[(uint32_t)4U * i + (uint32_t)2U];
+    uint64_t t212 = p[(uint32_t)4U * i + (uint32_t)2U];
+    uint64_t *res_i2 = tempBuffer + (uint32_t)4U * i + (uint32_t)2U;
+    c = Lib_IntTypes_Intrinsics_sub_borrow_u64(c, t11, t212, res_i2);
+    uint64_t t12 = x_[(uint32_t)4U * i + (uint32_t)3U];
+    uint64_t t21 = p[(uint32_t)4U * i + (uint32_t)3U];
+    uint64_t *res_i = tempBuffer + (uint32_t)4U * i + (uint32_t)3U;
+    c = Lib_IntTypes_Intrinsics_sub_borrow_u64(c, t12, t21, res_i);
+  }
+  for (uint32_t i = len4 / (uint32_t)4U * (uint32_t)4U; i < len4; i++)
+  {
+    uint64_t t1 = x_[i];
+    uint64_t t21 = p[i];
+    uint64_t *res_i = tempBuffer + i;
+    c = Lib_IntTypes_Intrinsics_sub_borrow_u64(c, t1, t21, res_i);
+  }
+  uint64_t r = c;
+  uint64_t carry0 = r;
+  uint64_t
+  carry =
+    Lib_IntTypes_Intrinsics_sub_borrow_u64(carry0,
+      cin,
+      (uint64_t)0U,
+      &tempBufferForSubborrow);
+  cmovznz4_p256(carry, tempBuffer, x_, result);
+}
+
+static inline void
 point_add_mixed_p256(uint64_t *p, uint64_t *q, uint64_t *result, uint64_t *tempBuffer)
 {
   uint64_t *t12 = tempBuffer;
@@ -2363,15 +2504,140 @@ point_add_mixed_p256(uint64_t *p, uint64_t *q, uint64_t *result, uint64_t *tempB
   uint64_t *z1Square = t4 + (uint32_t)4U;
   uint64_t *z2Cube = t4 + (uint32_t)8U;
   uint64_t *z1Cube = t4 + (uint32_t)12U;
-  z2Square[0U] = (uint64_t)0x000000300000000U;
-  z2Square[1U] = (uint64_t)0x00000001FFFFFFFEU;
-  z2Square[2U] = (uint64_t)0xFFFFFFFD00000002U;
-  z2Square[3U] = (uint64_t)0xFFFFFFFE00000003U;
-  z2Cube[0U] = (uint64_t)0x0000000CFFFFFFF7U;
-  z2Cube[1U] = (uint64_t)0xFFFFFFF800000007U;
-  z2Cube[2U] = (uint64_t)0xFFFFFFFB0000000FU;
-  z2Cube[3U] = (uint64_t)0x00000005FFFFFFFFU;
+  montgomery_multiplication_buffer_by_one_mixed_p256(z2Square);
   montgomery_square_buffer_dh_p256(pZ, z1Square);
+  uint32_t len0 = (uint32_t)4U;
+  KRML_CHECK_SIZE(sizeof (uint64_t), (uint32_t)2U * len0);
+  uint64_t t0[(uint32_t)2U * len0];
+  memset(t0, 0U, (uint32_t)2U * len0 * sizeof (uint64_t));
+  uint64_t *t_low0 = t0;
+  memcpy(t_low0, z2Square, len0 * sizeof (uint64_t));
+  uint32_t len10 = (uint32_t)4U;
+  KRML_CHECK_SIZE(sizeof (uint64_t), (uint32_t)2U * len10);
+  uint64_t t20[(uint32_t)2U * len10];
+  memset(t20, 0U, (uint32_t)2U * len10 * sizeof (uint64_t));
+  for (uint32_t i0 = (uint32_t)0U; i0 < len10; i0++)
+  {
+    uint64_t t10 = t0[0U];
+    uint64_t *uu____0 = t20;
+    uint32_t len30 = (uint32_t)4U;
+    for (uint32_t i = (uint32_t)0U; i < len30; i++)
+    {
+      uu____0[i] = (uint64_t)0U;
+    }
+    uint64_t *uu____1 = t20 + (uint32_t)4U;
+    uint32_t len31 = (uint32_t)4U;
+    for (uint32_t i = (uint32_t)0U; i < len31; i++)
+    {
+      uu____1[i] = (uint64_t)0U;
+    }
+    uint64_t temp = (uint64_t)0U;
+    uint64_t f0 = (uint64_t)0xffffffffffffffffU;
+    uint64_t f1 = (uint64_t)0xffffffffU;
+    uint64_t f3 = (uint64_t)0xffffffff00000001U;
+    uint64_t *o0 = t20;
+    uint64_t *o1 = t20 + (uint32_t)1U;
+    uint64_t *o2 = t20 + (uint32_t)2U;
+    uint64_t *o3 = t20 + (uint32_t)3U;
+    uint64_t *o4 = t20 + (uint32_t)4U;
+    mul64(f0, t10, o0, &temp);
+    uint64_t h0 = temp;
+    mul64(f1, t10, o1, &temp);
+    uint64_t l = o1[0U];
+    uint64_t c1 = Lib_IntTypes_Intrinsics_add_carry_u64((uint64_t)0U, l, h0, o1);
+    uint64_t h = temp;
+    o2[0U] = h + c1;
+    mul64(f3, t10, o3, o4);
+    uint32_t len32 = (uint32_t)4U * (uint32_t)2U;
+    uint64_t c = (uint64_t)0U;
+    for (uint32_t i = (uint32_t)0U; i < len32 / (uint32_t)4U * (uint32_t)4U / (uint32_t)4U; i++)
+    {
+      uint64_t t1 = t0[(uint32_t)4U * i];
+      uint64_t t210 = t20[(uint32_t)4U * i];
+      uint64_t *res_i0 = t20 + (uint32_t)4U * i;
+      c = Lib_IntTypes_Intrinsics_add_carry_u64(c, t1, t210, res_i0);
+      uint64_t t11 = t0[(uint32_t)4U * i + (uint32_t)1U];
+      uint64_t t211 = t20[(uint32_t)4U * i + (uint32_t)1U];
+      uint64_t *res_i1 = t20 + (uint32_t)4U * i + (uint32_t)1U;
+      c = Lib_IntTypes_Intrinsics_add_carry_u64(c, t11, t211, res_i1);
+      uint64_t t13 = t0[(uint32_t)4U * i + (uint32_t)2U];
+      uint64_t t212 = t20[(uint32_t)4U * i + (uint32_t)2U];
+      uint64_t *res_i2 = t20 + (uint32_t)4U * i + (uint32_t)2U;
+      c = Lib_IntTypes_Intrinsics_add_carry_u64(c, t13, t212, res_i2);
+      uint64_t t14 = t0[(uint32_t)4U * i + (uint32_t)3U];
+      uint64_t t21 = t20[(uint32_t)4U * i + (uint32_t)3U];
+      uint64_t *res_i = t20 + (uint32_t)4U * i + (uint32_t)3U;
+      c = Lib_IntTypes_Intrinsics_add_carry_u64(c, t14, t21, res_i);
+    }
+    for (uint32_t i = len32 / (uint32_t)4U * (uint32_t)4U; i < len32; i++)
+    {
+      uint64_t t1 = t0[i];
+      uint64_t t21 = t20[i];
+      uint64_t *res_i = t20 + i;
+      c = Lib_IntTypes_Intrinsics_add_carry_u64(c, t1, t21, res_i);
+    }
+    uint64_t carry = c;
+    uint32_t len3 = (uint32_t)7U;
+    for (uint32_t i = (uint32_t)0U; i < len3; i++)
+    {
+      uint64_t elem = t20[(uint32_t)1U + i];
+      t0[i] = elem;
+    }
+    t0[len3] = carry;
+  }
+  uint32_t len2 = (uint32_t)4U;
+  uint64_t cin = t0[len2];
+  uint64_t *x_0 = t0;
+  uint32_t len30 = (uint32_t)4U;
+  KRML_CHECK_SIZE(sizeof (uint64_t), len30);
+  uint64_t tempBuffer1[len30];
+  memset(tempBuffer1, 0U, len30 * sizeof (uint64_t));
+  uint64_t tempBufferForSubborrow0 = (uint64_t)0U;
+  uint64_t
+  p10[4U] =
+    {
+      (uint64_t)0xffffffffffffffffU,
+      (uint64_t)0xffffffffU,
+      (uint64_t)0U,
+      (uint64_t)0xffffffff00000001U
+    };
+  uint32_t len40 = (uint32_t)4U;
+  uint64_t c0 = (uint64_t)0U;
+  for (uint32_t i = (uint32_t)0U; i < len40 / (uint32_t)4U * (uint32_t)4U / (uint32_t)4U; i++)
+  {
+    uint64_t t1 = x_0[(uint32_t)4U * i];
+    uint64_t t210 = p10[(uint32_t)4U * i];
+    uint64_t *res_i0 = tempBuffer1 + (uint32_t)4U * i;
+    c0 = Lib_IntTypes_Intrinsics_sub_borrow_u64(c0, t1, t210, res_i0);
+    uint64_t t10 = x_0[(uint32_t)4U * i + (uint32_t)1U];
+    uint64_t t211 = p10[(uint32_t)4U * i + (uint32_t)1U];
+    uint64_t *res_i1 = tempBuffer1 + (uint32_t)4U * i + (uint32_t)1U;
+    c0 = Lib_IntTypes_Intrinsics_sub_borrow_u64(c0, t10, t211, res_i1);
+    uint64_t t11 = x_0[(uint32_t)4U * i + (uint32_t)2U];
+    uint64_t t212 = p10[(uint32_t)4U * i + (uint32_t)2U];
+    uint64_t *res_i2 = tempBuffer1 + (uint32_t)4U * i + (uint32_t)2U;
+    c0 = Lib_IntTypes_Intrinsics_sub_borrow_u64(c0, t11, t212, res_i2);
+    uint64_t t13 = x_0[(uint32_t)4U * i + (uint32_t)3U];
+    uint64_t t21 = p10[(uint32_t)4U * i + (uint32_t)3U];
+    uint64_t *res_i = tempBuffer1 + (uint32_t)4U * i + (uint32_t)3U;
+    c0 = Lib_IntTypes_Intrinsics_sub_borrow_u64(c0, t13, t21, res_i);
+  }
+  for (uint32_t i = len40 / (uint32_t)4U * (uint32_t)4U; i < len40; i++)
+  {
+    uint64_t t1 = x_0[i];
+    uint64_t t21 = p10[i];
+    uint64_t *res_i = tempBuffer1 + i;
+    c0 = Lib_IntTypes_Intrinsics_sub_borrow_u64(c0, t1, t21, res_i);
+  }
+  uint64_t r0 = c0;
+  uint64_t carry0 = r0;
+  uint64_t
+  carry =
+    Lib_IntTypes_Intrinsics_sub_borrow_u64(carry0,
+      cin,
+      (uint64_t)0U,
+      &tempBufferForSubborrow0);
+  cmovznz4_p256(carry, tempBuffer1, x_0, z2Cube);
   montgomery_multiplication_buffer_dh_p256(z1Square, pZ, z1Cube);
   montgomery_multiplication_buffer_dh_p256(z2Square, pX, u10);
   montgomery_multiplication_buffer_dh_p256(z1Square, qX, u20);
@@ -2383,11 +2649,11 @@ point_add_mixed_p256(uint64_t *p, uint64_t *q, uint64_t *result, uint64_t *tempB
   uint64_t *s11 = t12 + (uint32_t)24U;
   uint64_t *s2 = t12 + (uint32_t)28U;
   uint64_t *h = t12 + (uint32_t)32U;
-  uint64_t *r0 = t12 + (uint32_t)36U;
+  uint64_t *r1 = t12 + (uint32_t)36U;
   uint64_t *uh0 = t12 + (uint32_t)40U;
   uint64_t *hCube0 = t12 + (uint32_t)44U;
   felem_sub_p256(u2, u1, h);
-  felem_sub_p256(s2, s11, r0);
+  felem_sub_p256(s2, s11, r1);
   montgomery_square_buffer_dh_p256(h, temp);
   montgomery_multiplication_buffer_dh_p256(temp, u1, uh0);
   montgomery_multiplication_buffer_dh_p256(temp, h, hCube0);
@@ -2416,30 +2682,30 @@ point_add_mixed_p256(uint64_t *p, uint64_t *q, uint64_t *result, uint64_t *tempB
   uint64_t *z1 = p + (uint32_t)8U;
   uint64_t *z3 = t5 + (uint32_t)8U;
   uint64_t *z1z2 = t5 + (uint32_t)12U;
-  uint32_t len0 = (uint32_t)4U;
-  KRML_CHECK_SIZE(sizeof (uint64_t), (uint32_t)2U * len0);
-  uint64_t t[(uint32_t)2U * len0];
-  memset(t, 0U, (uint32_t)2U * len0 * sizeof (uint64_t));
+  uint32_t len5 = (uint32_t)4U;
+  KRML_CHECK_SIZE(sizeof (uint64_t), (uint32_t)2U * len5);
+  uint64_t t[(uint32_t)2U * len5];
+  memset(t, 0U, (uint32_t)2U * len5 * sizeof (uint64_t));
   uint64_t *t_low = t;
-  memcpy(t_low, z1, len0 * sizeof (uint64_t));
-  uint32_t len1 = (uint32_t)4U;
-  KRML_CHECK_SIZE(sizeof (uint64_t), (uint32_t)2U * len1);
-  uint64_t t2[(uint32_t)2U * len1];
-  memset(t2, 0U, (uint32_t)2U * len1 * sizeof (uint64_t));
-  for (uint32_t i0 = (uint32_t)0U; i0 < len1; i0++)
+  memcpy(t_low, z1, len5 * sizeof (uint64_t));
+  uint32_t len11 = (uint32_t)4U;
+  KRML_CHECK_SIZE(sizeof (uint64_t), (uint32_t)2U * len11);
+  uint64_t t2[(uint32_t)2U * len11];
+  memset(t2, 0U, (uint32_t)2U * len11 * sizeof (uint64_t));
+  for (uint32_t i0 = (uint32_t)0U; i0 < len11; i0++)
   {
     uint64_t t10 = t[0U];
-    uint64_t *uu____0 = t2;
-    uint32_t len30 = (uint32_t)4U;
-    for (uint32_t i = (uint32_t)0U; i < len30; i++)
-    {
-      uu____0[i] = (uint64_t)0U;
-    }
-    uint64_t *uu____1 = t2 + (uint32_t)4U;
+    uint64_t *uu____2 = t2;
     uint32_t len31 = (uint32_t)4U;
     for (uint32_t i = (uint32_t)0U; i < len31; i++)
     {
-      uu____1[i] = (uint64_t)0U;
+      uu____2[i] = (uint64_t)0U;
+    }
+    uint64_t *uu____3 = t2 + (uint32_t)4U;
+    uint32_t len32 = (uint32_t)4U;
+    for (uint32_t i = (uint32_t)0U; i < len32; i++)
+    {
+      uu____3[i] = (uint64_t)0U;
     }
     uint64_t temp0 = (uint64_t)0U;
     uint64_t f0 = (uint64_t)0xffffffffffffffffU;
@@ -2458,9 +2724,9 @@ point_add_mixed_p256(uint64_t *p, uint64_t *q, uint64_t *result, uint64_t *tempB
     uint64_t h3 = temp0;
     o2[0U] = h3 + c1;
     mul64(f3, t10, o3, o4);
-    uint32_t len32 = (uint32_t)4U * (uint32_t)2U;
+    uint32_t len33 = (uint32_t)4U * (uint32_t)2U;
     uint64_t c = (uint64_t)0U;
-    for (uint32_t i = (uint32_t)0U; i < len32 / (uint32_t)4U * (uint32_t)4U / (uint32_t)4U; i++)
+    for (uint32_t i = (uint32_t)0U; i < len33 / (uint32_t)4U * (uint32_t)4U / (uint32_t)4U; i++)
     {
       uint64_t t1 = t[(uint32_t)4U * i];
       uint64_t t210 = t2[(uint32_t)4U * i];
@@ -2479,29 +2745,29 @@ point_add_mixed_p256(uint64_t *p, uint64_t *q, uint64_t *result, uint64_t *tempB
       uint64_t *res_i = t2 + (uint32_t)4U * i + (uint32_t)3U;
       c = Lib_IntTypes_Intrinsics_add_carry_u64(c, t14, t21, res_i);
     }
-    for (uint32_t i = len32 / (uint32_t)4U * (uint32_t)4U; i < len32; i++)
+    for (uint32_t i = len33 / (uint32_t)4U * (uint32_t)4U; i < len33; i++)
     {
       uint64_t t1 = t[i];
       uint64_t t21 = t2[i];
       uint64_t *res_i = t2 + i;
       c = Lib_IntTypes_Intrinsics_add_carry_u64(c, t1, t21, res_i);
     }
-    uint64_t carry = c;
+    uint64_t carry1 = c;
     uint32_t len3 = (uint32_t)7U;
     for (uint32_t i = (uint32_t)0U; i < len3; i++)
     {
       uint64_t elem = t2[(uint32_t)1U + i];
       t[i] = elem;
     }
-    t[len3] = carry;
+    t[len3] = carry1;
   }
-  uint32_t len2 = (uint32_t)4U;
-  uint64_t cin = t[len2];
+  uint32_t len20 = (uint32_t)4U;
+  uint64_t cin0 = t[len20];
   uint64_t *x_ = t;
   uint32_t len3 = (uint32_t)4U;
   KRML_CHECK_SIZE(sizeof (uint64_t), len3);
-  uint64_t tempBuffer1[len3];
-  memset(tempBuffer1, 0U, len3 * sizeof (uint64_t));
+  uint64_t tempBuffer10[len3];
+  memset(tempBuffer10, 0U, len3 * sizeof (uint64_t));
   uint64_t tempBufferForSubborrow = (uint64_t)0U;
   uint64_t
   p1[4U] =
@@ -2517,88 +2783,92 @@ point_add_mixed_p256(uint64_t *p, uint64_t *q, uint64_t *result, uint64_t *tempB
   {
     uint64_t t1 = x_[(uint32_t)4U * i];
     uint64_t t210 = p1[(uint32_t)4U * i];
-    uint64_t *res_i0 = tempBuffer1 + (uint32_t)4U * i;
+    uint64_t *res_i0 = tempBuffer10 + (uint32_t)4U * i;
     c = Lib_IntTypes_Intrinsics_sub_borrow_u64(c, t1, t210, res_i0);
     uint64_t t10 = x_[(uint32_t)4U * i + (uint32_t)1U];
     uint64_t t211 = p1[(uint32_t)4U * i + (uint32_t)1U];
-    uint64_t *res_i1 = tempBuffer1 + (uint32_t)4U * i + (uint32_t)1U;
+    uint64_t *res_i1 = tempBuffer10 + (uint32_t)4U * i + (uint32_t)1U;
     c = Lib_IntTypes_Intrinsics_sub_borrow_u64(c, t10, t211, res_i1);
     uint64_t t11 = x_[(uint32_t)4U * i + (uint32_t)2U];
     uint64_t t212 = p1[(uint32_t)4U * i + (uint32_t)2U];
-    uint64_t *res_i2 = tempBuffer1 + (uint32_t)4U * i + (uint32_t)2U;
+    uint64_t *res_i2 = tempBuffer10 + (uint32_t)4U * i + (uint32_t)2U;
     c = Lib_IntTypes_Intrinsics_sub_borrow_u64(c, t11, t212, res_i2);
     uint64_t t13 = x_[(uint32_t)4U * i + (uint32_t)3U];
     uint64_t t21 = p1[(uint32_t)4U * i + (uint32_t)3U];
-    uint64_t *res_i = tempBuffer1 + (uint32_t)4U * i + (uint32_t)3U;
+    uint64_t *res_i = tempBuffer10 + (uint32_t)4U * i + (uint32_t)3U;
     c = Lib_IntTypes_Intrinsics_sub_borrow_u64(c, t13, t21, res_i);
   }
   for (uint32_t i = len4 / (uint32_t)4U * (uint32_t)4U; i < len4; i++)
   {
     uint64_t t1 = x_[i];
     uint64_t t21 = p1[i];
-    uint64_t *res_i = tempBuffer1 + i;
+    uint64_t *res_i = tempBuffer10 + i;
     c = Lib_IntTypes_Intrinsics_sub_borrow_u64(c, t1, t21, res_i);
   }
-  uint64_t r1 = c;
-  uint64_t carry0 = r1;
+  uint64_t r10 = c;
+  uint64_t carry00 = r10;
   uint64_t
-  carry =
-    Lib_IntTypes_Intrinsics_sub_borrow_u64(carry0,
-      cin,
+  carry1 =
+    Lib_IntTypes_Intrinsics_sub_borrow_u64(carry00,
+      cin0,
       (uint64_t)0U,
       &tempBufferForSubborrow);
-  cmovznz4_p256(carry, tempBuffer1, x_, z1z2);
+  cmovznz4_p256(carry1, tempBuffer10, x_, z1z2);
   montgomery_multiplication_buffer_dh_p256(z1z2, h0, z3);
-
-
   uint64_t *x3_out = t5;
   uint64_t *y3_out = t5 + (uint32_t)4U;
   uint64_t *z3_out = t5 + (uint32_t)8U;
-
-
-  uint64_t *z = q + (uint32_t)4U;
-  uint64_t tmp = (uint64_t)18446744073709551615U;
+  uint64_t *z = p + (uint32_t)8U;
+  uint64_t tmp1 = (uint64_t)18446744073709551615U;
   uint32_t len = (uint32_t)4U;
   for (uint32_t i = (uint32_t)0U; i < len; i++)
   {
     uint64_t a_i = z[i];
     uint64_t r_i = FStar_UInt64_eq_mask(a_i, (uint64_t)0U);
+    uint64_t tmp0 = tmp1;
+    tmp1 = r_i & tmp0;
+  }
+  uint64_t mask = tmp1;
+  uint64_t *p_x0 = q;
+  uint64_t *p_y0 = q + (uint32_t)4U;
+  uint64_t *p_z0 = q + (uint32_t)8U;
+  copy_conditional_p256_l(x3_out, p_x0, mask);
+  copy_conditional_p256_l(y3_out, p_y0, mask);
+  copy_conditional_p256_l(z3_out, p_z0, mask);
+  uint32_t len6 = (uint32_t)4U;
+  uint64_t *x = q;
+  uint64_t *y = q + len6;
+  uint64_t tmp2 = (uint64_t)18446744073709551615U;
+  uint32_t len12 = (uint32_t)4U;
+  for (uint32_t i = (uint32_t)0U; i < len12; i++)
+  {
+    uint64_t a_i = x[i];
+    uint64_t r_i = FStar_UInt64_eq_mask(a_i, (uint64_t)0U);
+    uint64_t tmp0 = tmp2;
+    tmp2 = r_i & tmp0;
+  }
+  uint64_t xZero = tmp2;
+  uint64_t tmp = (uint64_t)18446744073709551615U;
+  uint32_t len1 = (uint32_t)4U;
+  for (uint32_t i = (uint32_t)0U; i < len1; i++)
+  {
+    uint64_t a_i = y[i];
+    uint64_t r_i = FStar_UInt64_eq_mask(a_i, (uint64_t)0U);
     uint64_t tmp0 = tmp;
     tmp = r_i & tmp0;
   }
-
-  uint64_t mask = tmp;
-
-
+  uint64_t yZero = tmp;
+  uint64_t mask0 = xZero & yZero;
   uint64_t *p_x = p;
   uint64_t *p_y = p + (uint32_t)4U;
   uint64_t *p_z = p + (uint32_t)8U;
-
-  printf("%s\n", "Before");
-  printU(t5, 12);
-
-  copy_conditional_p256_l(x3_out, p_x, mask);
-  copy_conditional_p256_l(y3_out, p_y, mask);
-  copy_conditional_p256_l(z3_out, p_z, mask);
-
-  printf("%s\n", "After");
-  printU(t5, 12);
-
+  copy_conditional_p256_l(x3_out, p_x, mask0);
+  copy_conditional_p256_l(y3_out, p_y, mask0);
+  copy_conditional_p256_l(z3_out, p_z, mask0);
   memcpy(result, x3_out, (uint32_t)4U * sizeof (uint64_t));
   memcpy(result + (uint32_t)4U, y3_out, (uint32_t)4U * sizeof (uint64_t));
   memcpy(result + (uint32_t)8U, z3_out, (uint32_t)4U * sizeof (uint64_t));
 }
-
-
-#include <inttypes.h>
-void printU(uint64_t* t, int len)
-{
-  for (int i = 0; i< len; i++) {
-    printf("%016llX ", t[i]);  
-  }
-  printf("\n");
-}
-
 
 static const
 uint64_t
@@ -2746,7 +3016,7 @@ static inline void point_double_p384(uint64_t *p, uint64_t *result, uint64_t *te
   felem_sub_p384(y3, eightGamma, y3);
 }
 
-static void getPointPrecomputedMixed_p256(uint8_t *scalar, uint32_t i, uint64_t *pointToAdd)
+static inline void getPointPrecomputedMixed_p256(uint8_t *scalar, uint32_t i, uint64_t *pointToAdd)
 {
   uint32_t half = i >> (uint32_t)1U;
   uint32_t word = (uint32_t)scalar[half];
